Unused/TableauFlipEdgeWF.lean
@@ -1,0 +1,38 @@
+
+/-- This no longer holds, now that we continue at loaded non-lprs.
+Was only used for flipEdge.wellFounded which now uses a different argument. -/
+lemma PathIn.mem_history_multisetEqTo_then_lrep {tab : Tableau Hist X} (p : PathIn tab) :
+    (∃ Y ∈ (tabAt p).1, Y.multisetEqTo (nodeAt p)) → (tabAt p).2.2.isLrep := by
+  rintro ⟨Y, h1, h2⟩
+  generalize h : tabAt p = tp
+  rcases tp with ⟨H, Z, t⟩
+  simp [nodeAt] at h2
+  rw [h] at h2
+  cases t
+  case loc _ _   nrep _ => sorry
+    -- exact nrep ⟨Y, by have := Sequent.setEqTo_of_multisetEqTo; aesop⟩
+  case pdl _ _ _ nrep _ => sorry
+    -- exact nrep ⟨Y, by have := Sequent.setEqTo_of_multisetEqTo; aesop⟩
+  case lrep             => simp [Tableau.isLrep]
+
+lemma single_of_transgen {α} {r} {a c : α} : Relation.TransGen r a c → ∃ b, r a b := by
+  intro h
+  induction h
+  case single b e => use b
+  case tail d e ih => assumption
+
+instance flipEdge.instIsIrrefl : @Std.Irrefl (PathIn tab) (Relation.TransGen (flip edge)) := by
+  constructor
+  intro p p_p
+  rw [Relation.transGen_swap] at p_p
+  have p_in_Hist_p := edge_TransGen_then_mem_History p_p
+  have := PathIn.mem_history_multisetEqTo_then_lrep p ⟨nodeAt p, by simpa⟩
+  rcases (single_of_transgen p_p) with ⟨_,   ⟨_, _, _, _, _, _, _, _, h, _⟩
+                                           | ⟨_, _, _, _, _, _, _, h, _⟩⟩
+  <;> rw [h] at this <;> contradiction
+
+/-- The `flip edge` relation in a tableau is well-founded. -/
+theorem flipEdge.wellFounded :
+  WellFounded (flip (@edge _ _ tab)) := by
+  apply Finite.wellfounded_of_irrefl_TC _ flipEdge.instIsIrrefl
+-/
